Halfway through Fw with unified env

dev/stlc_tabs_topr_pts_wip1.v
@@ -42,7 +42,7 @@ Inductive tm : Type :=
   | TBox   : tm
 
   | TBool  : tm
-  | TVar   : id -> tm
+(*  | TVar   : id -> tm   <--- now using tvar x! (alias below) *)
   | TFun   : tm -> tm -> tm  
   | TAll   : tm -> tm -> tm
 
@@ -65,11 +65,17 @@ Inductive vl: Type :=
   | vtabs  :  list vl -> tm -> vl
 .
 
+Definition ty := tm.
+Definition TVar x := tvar x.
+
+
+Definition binding := (bool * tm)%type.
+
 (* the interpretation of kind, which defines the set at * *)
 Definition tpe := vl -> Prop.
 Definition venv := list vl.
-Definition tenv := list tm. (*ty*)
-Definition kenv := list tm. (*ty*)
+Definition tenv := list binding.
+Definition kenv := tenv.
 
 #[global] Hint Unfold venv.
 #[global] Hint Unfold tenv.
@@ -109,7 +115,7 @@ Fixpoint teval(n: nat)(env: venv)(t: tm){struct n}: option (option vl) :=
           | Some (Some (vbool _)) => Some None
           | Some (Some (vabs env2 ey)) => Some None
           | Some (Some (vtabs env2 ey)) =>
-              teval n env2 ey
+              teval n ((vbool false)::env2) ey
           end
       | _ => Some None
       end
@@ -125,19 +131,15 @@ Fixpoint splice (i: nat) (n:nat) (t: tm): tm :=
   | TStar         => TStar
   | TBox          => TBox
   | TBool         => TBool
-  | TVar x        => TVar (if x <? i then x else x + n)
+  | tvar x        => tvar (if x <? i then x else x + n)
   | TFun t1 t2    => TFun (splice i n t1) (splice i n t2)
-  | TAll k t      => TAll k (splice i n t)
-(*| TKArr t1 t2   => TKArr (splice i n t1) (splice i n t2)
-  | TTAbs k t     => TTAbs k (splice i n t)
-  | TTApp t1 t2   => TTApp (splice i n t1) (splice i n t2) *)
+  | TAll k t      => TAll (splice i n k) (splice i n t)
   | ttrue         => ttrue
   | tfalse        => tfalse
-  | tvar x        => tvar x
   | tapp t1 t2    => tapp (splice i n t1) (splice i n t2)
   | tabs t1       => tabs (splice i n t1)
   | ttapp t1 t2   => ttapp (splice i n t1) (splice i n t2)
-  | ttabs t1 t2   => ttabs t1(*?*) (splice i n t2)
+  | ttabs t1 t2   => ttabs (splice i n t1) (splice i n t2)
   end.
 
 Fixpoint subst (t: tm) (i: nat) (u:tm): tm :=
@@ -145,20 +147,43 @@ Fixpoint subst (t: tm) (i: nat) (u:tm): tm :=
   | TStar         => TStar
   | TBox          => TBox
   | TBool         => TBool
-  | TVar x        => if Nat.eq_dec x i then u else TVar (if x <? i then x else x-1)
+  | tvar x        => if Nat.eq_dec x i then u else tvar (if x <? i then x else x-1)
   | TFun t1 t2    => TFun (subst t1 i u) (subst t2 i u)
-  | TAll k t      => TAll k (subst t i (splice i 1 u))
-(*| TKArr t1 t2   => TKArr (subst t1 i u) (subst t2 i u)
-  | TTAbs k t     => TTAbs k (subst t i (splice i 1 u))
-  | TTApp t1 t2   => TTApp (subst t1 i u) (subst t2 i u)*)
+  | TAll k t      => TAll (subst k i u) (subst t i (splice i 1 u))
   | ttrue         => ttrue
   | tfalse        => tfalse
-  | tvar x        => tvar x
   | tapp t1 t2    => tapp (subst t1 i u) (subst t2 i u)
-  | tabs t1       => tabs (subst t1 i u)
+  | tabs t1       => tabs (subst t1 i (splice i 1 u))
   | ttapp t1 t2   => ttapp (subst t1 i u) (subst t2 i u)
-  | ttabs t1 t2   => ttabs t1(*?*) (subst t2 i (splice i 1 u))
-end.
+  | ttabs t1 t2   => ttabs (subst t1 i u) (subst t2 i (splice i 1 u))
+  end.
+
+Definition bsplice i n (b: binding) : binding :=
+  match b with
+  | (is_ty, T) => (is_ty, splice i n T)
+  end.
+
+
+
+Definition bind_tm (T: tm) : binding := (false, T).
+Definition bind_ty (K: tm) : binding := (true, K).
+Definition ext (b: binding) (G: tenv) : tenv := map (bsplice (length G) 1) (b :: G).
+
+(* multi-extension: fold ext over a list of bindings *)
+Fixpoint mext (bs: list binding) (G: tenv) : tenv :=
+  match bs with
+  | [] => G
+  | b :: bs' => ext b (mext bs' G)
+  end.
+
+Lemma mext_length: forall bs G,
+    length (mext bs G) = length bs + length G.
+Proof.
+  induction bs; intros; simpl.
+  - lia.
+  - unfold ext. rewrite map_length. simpl. rewrite IHbs. lia.
+Qed.
+
 
 (* ---------- LR definitions for types : kinds  ---------- *)
 
@@ -168,21 +193,21 @@ Inductive has_kind J : tm -> tm -> Type :=
 | k_bool:
     has_kind J TBool TStar
 | k_var: forall x K,
-    indexr x J = Some K ->
+    indexr x J = Some (true, K) ->
     has_kind J (TVar x) K
 | k_fun: forall T1 T2, (* (term -> term): type *)
     has_kind J T1 TStar ->
     has_kind J T2 TStar ->
     has_kind J (TFun T1 T2) TStar
 | k_all: forall K1 T2, (* (type -> term): type *)
-    has_kind (K1::J) T2 TStar ->
+    has_kind (ext (bind_ty K1) J) T2 TStar ->
     has_kind J (TAll K1 T2) TStar
 | k_karr: forall K1 K2, (* (type -> type): kind *)
     has_kind J K1 TBox ->
     has_kind J K2 TBox ->
     has_kind J (TFun K1 K2) TBox
 | k_tabs: forall K1 T2 K2,
-    has_kind (K1::J) T2 K2 ->
+    has_kind (ext (bind_ty K1) J) T2 K2 ->
     has_kind J (ttabs K1 T2) (TFun K1 K2) (* (tabs K1 T2) (TPi K1 K2) *)
 | k_tapp: forall TF TX K1 K2,
     has_kind J TF (TFun K1 K2) ->
@@ -190,8 +215,7 @@ Inductive has_kind J : tm -> tm -> Type :=
     has_kind J (ttapp TF TX) K2
 .
 
-(* note: we can either include kn in the definition, or derive it later *)
-Inductive eq_type : kenv -> tm -> tm -> Type :=
+Inductive eq_type : tenv -> tm -> tm -> Type :=
 | q_refl: forall J T,
     eq_type J T T
 | q_symm: forall J T1 T2,
@@ -206,10 +230,10 @@ Inductive eq_type : kenv -> tm -> tm -> Type :=
     eq_type J T2 T2' ->
     eq_type J (TFun T1 T2) (TFun T1' T2')
 | q_tall : forall J T2 T2' K1,
-    eq_type (K1::J) T2 T2' ->
+    eq_type (ext (bind_ty K1) J) T2 T2' ->
     eq_type J (TAll K1 T2) (TAll K1 T2')
 | q_tabs: forall J T2 T2' K1,
-    eq_type (K1::J) T2 T2' ->
+    eq_type (ext (bind_ty K1) J) T2 T2' ->
     eq_type J (ttabs K1 T2) (ttabs K1 T2')
 | q_tapp: forall J T1 T2 T1' T2',
     eq_type J T1 T1' ->
@@ -220,39 +244,39 @@ Inductive eq_type : kenv -> tm -> tm -> Type :=
     eq_type J (ttapp (ttabs K1 T2) T1) (subst T2 (length J) T1)
 .
 
-Inductive has_type : tenv -> kenv -> tm -> tm -> Type :=
-| t_true: forall G J,
-    has_type G J ttrue TBool
-| t_false: forall G J,
-    has_type G J tfalse TBool
-| t_var: forall x G J T,
-    indexr x G = Some T ->
-    has_type G J (tvar x) T
+Inductive has_type : tenv -> tm -> tm -> Type :=
+| t_true: forall G,
+    has_type G ttrue TBool
+| t_false: forall G,
+    has_type G tfalse TBool
+| t_var: forall x G T,
+    indexr x G = Some (false, T) ->
+    has_type G (tvar x) T
 
-| t_abs: forall G J t T1 T2,
-    has_type (T1::G) J t T2 ->
-    has_kind J T1 TStar ->
-    has_kind J T2 TStar ->
-    has_type G J (tabs t) (TFun T1 T2)
-| t_app: forall G J f t T1 T2,
-    has_type G J f (TFun T1 T2) ->
-    has_type G J t T1 ->
-    has_type G J (tapp f t) T2
+| t_abs: forall G t T1 T2,
+    has_type (ext (bind_tm T1) G) t (splice (length G) 1 T2) ->
+    has_kind G T1 TStar ->
+    has_kind G T2 TStar ->
+    has_type G (tabs t) (TFun T1 T2)
+| t_app: forall G f t T1 T2,
+    has_type G f (TFun T1 T2) ->
+    has_type G t T1 ->
+    has_type G (tapp f t) T2
 
-| t_tabs: forall G J t K1 T2,
-    has_type (map (splice (length J) 1) G) (K1::J) t T2 ->
-    has_kind (K1::J) T2 TStar ->
-    has_type G J (ttabs K1 t) (TAll K1 T2)
-| t_tapp: forall G J f K1 T1 T2,
-    has_type G J f (TAll K1 T2) ->
-    has_kind J T1 K1 ->
-    has_type G J (ttapp f T1) (subst T2 (length J) T1)
+| t_tabs: forall G t K1 T2,
+    has_type (ext (bind_ty K1) G) t T2 ->
+    has_kind (ext (bind_ty K1) G) T2 TStar ->
+    has_type G (ttabs K1 t) (TAll K1 T2)
+| t_tapp: forall G f K1 T1 T2,
+    has_type G f (TAll K1 T2) ->
+    has_kind G T1 K1 ->
+    has_type G (ttapp f T1) (subst T2 (length G) T1)
 
-| t_equiv: forall G J t T1 T2,
-    has_type G J t T1 ->
-    eq_type J T1 T2 ->
-    has_kind J T2 TStar ->
-    has_type G J t T2
+| t_equiv: forall G t T1 T2,
+    has_type G t T1 ->
+    eq_type G T1 T2 ->
+    has_kind G T2 TStar ->
+    has_type G t T2
 .
 
 #[export] Hint Constructors tm: core.
@@ -283,6 +307,17 @@ Proof.
        eapply indexr_var_some in H. destruct H. eauto. }
   remember (indexr x M). destruct o. inversion H.
   eexists. intuition. inversion H.
+Qed.
+
+Lemma indexr_map'': forall {A B} (M: list A) x v (f: A -> B),
+    indexr x (map f M) = Some v ->
+    {v' & indexr x M = Some v' & v = f v'}.
+Proof.
+  intros. erewrite indexr_map in H.
+  2: { eapply indexr_var_some' in H. rewrite map_length in H.
+       eapply indexr_var_some in H. destruct H. eauto. }
+  remember (indexr x M). destruct o. inversion H.
+  eexists. eauto. eauto. inversion H.
 Qed.
 
 Lemma map_map: forall {A B C} (M: list A) (f: A -> B) (g: B -> C),
@@ -354,16 +389,15 @@ Lemma splice_acc: forall e1 a b c,
   splice a (c+b) e1.
 Proof.
   induction e1; intros; simpl; try reflexivity.
-  - bdestruct (i <? a); simpl; [bdestruct (i <? a); [auto | lia] | bdestruct (i+b <? a); [lia | f_equal; lia]].
   - rewrite IHe1_1, IHe1_2. auto.
-  - rewrite IHe1_2. auto.
   - rewrite IHe1_1, IHe1_2. auto.
-(*- rewrite IHe1_2. auto.
+  - bdestruct (i <? a); simpl.
+    + bdestruct (i <? a); [auto | lia].
+    + bdestruct (i + b <? a); [lia | f_equal; lia].
   - rewrite IHe1_1, IHe1_2. auto.
-  - rewrite IHe1_1, IHe1_2. auto.*)
   - rewrite IHe1. auto.
   - rewrite IHe1_1, IHe1_2. auto.
-  - rewrite IHe1_2. auto. 
+  - rewrite IHe1_1, IHe1_2. auto.
 Qed.
 
 Lemma splice_acc': forall e1 a b c,
@@ -371,36 +405,173 @@ Lemma splice_acc': forall e1 a b c,
   splice a (c+b) e1.
 Proof.
   induction e1; intros; simpl; try reflexivity.
+  - rewrite IHe1_1, IHe1_2. auto.
+  - rewrite IHe1_1, IHe1_2. auto.
   - bdestruct (i <? a); simpl.
     + bdestruct (i <? a); [|lia]. bdestruct (i <? b+a); [|lia]. auto.
     + bdestruct (i + b <? b + a); [lia|]. f_equal. lia.
   - rewrite IHe1_1, IHe1_2. auto.
-  - rewrite IHe1_2. auto.
-  - rewrite IHe1_1, IHe1_2. auto.
-(*- rewrite IHe1_2. auto.
-  - rewrite IHe1_1, IHe1_2. auto.
-  - rewrite IHe1_1, IHe1_2. auto.*)
   - rewrite IHe1. auto.
   - rewrite IHe1_1, IHe1_2. auto.
-  - rewrite IHe1_2. auto.
+  - rewrite IHe1_1, IHe1_2. auto.
 Qed.
 
 Lemma splice_zero: forall e1 a,
   (splice a 0 e1) = e1.
 Proof.
   intros. induction e1; simpl; try reflexivity.
+  - rewrite IHe1_1, IHe1_2. auto.
+  - rewrite IHe1_1, IHe1_2. auto.
   - bdestruct (i <? a); f_equal; lia.
   - rewrite IHe1_1, IHe1_2. auto.
-  - rewrite IHe1_2. auto.
-  - rewrite IHe1_1, IHe1_2. auto.
-(*- rewrite IHe1_2. auto.
-  - rewrite IHe1_1, IHe1_2. auto.
-  - rewrite IHe1_1, IHe1_2. auto.*)
   - rewrite IHe1. auto.
   - rewrite IHe1_1, IHe1_2. auto.
-  - rewrite IHe1_2. auto.
+  - rewrite IHe1_1, IHe1_2. auto.
 Qed.
 
+Lemma splice_var_comm: forall i a c b d,
+    a <= b ->
+    (if (if i <? b then i else i + d) <? a
+     then (if i <? b then i else i + d)
+     else (if i <? b then i else i + d) + c) =
+    (if (if i <? a then i else i + c) <? b + c
+     then (if i <? a then i else i + c)
+     else (if i <? a then i else i + c) + d).
+Proof.
+  intros.
+  bdestruct (i <? b); bdestruct (i <? a).
+  - bdestruct (i <? a); [|lia]. bdestruct (i <? b + c); [|lia]. lia.
+  - bdestruct (i <? a); [lia|].
+    destruct (Nat.ltb_spec (i+c) (b+c)); lia.
+  - lia.
+  - destruct (Nat.ltb_spec (i+d) a); [lia|].
+    destruct (Nat.ltb_spec (i+c) (b+c)); [lia|]. lia.
+Qed.
+
+Lemma splice_comm: forall e1 a c b d,
+    a <= b ->
+    splice a c (splice b d e1) = splice (b+c) d (splice a c e1).
+Proof.
+  induction e1; intros; simpl; try reflexivity;
+    try (rewrite IHe1_1, IHe1_2; auto; fail);
+    try (rewrite IHe1; auto; fail).
+  - f_equal. apply splice_var_comm. auto.
+Qed.
+
+Lemma bsplice_comm: forall (b: binding) a c i d,
+    a <= i ->
+    bsplice a c (bsplice i d b) = bsplice (i+c) d (bsplice a c b).
+Proof.
+  intros [? ?]; simpl; intros; f_equal; apply splice_comm; auto.
+Qed.
+
+Lemma map_bsplice_comm: forall G a c i d,
+    a <= i ->
+    map (bsplice a c) (map (bsplice i d) G) = map (bsplice (i+c) d) (map (bsplice a c) G).
+Proof.
+  induction G; simpl; intros; [auto|].
+  rewrite bsplice_comm; auto. f_equal. apply IHG; auto.
+Qed.
+
+Lemma ext_map_bsplice: forall b n m G,
+    n <= m ->
+    m = length G ->
+    map (bsplice n 1) (bsplice m 1 b :: map (bsplice m 1) G) =
+    map (bsplice (m+1) 1) (bsplice n 1 b :: map (bsplice n 1) G).
+Proof.
+  intros. simpl. f_equal.
+  - apply bsplice_comm; auto.
+  - apply map_bsplice_comm; auto.
+Qed.
+
+(* key lemma: when IH uses bsplice m 1 K1 as weakening binding,
+   the double-map on the full list commutes via map_bsplice_comm *)
+Lemma weaken_ext_comm: forall b J' J K1,
+    let n := length J in
+    let m := length (J' ++ J) in
+    map (bsplice n 1) (map (bsplice m 1) (b :: J' ++ K1 :: J)) =
+    map (bsplice (m+1) 1) (map (bsplice n 1) (b :: J' ++ K1 :: J)).
+Proof.
+  intros. subst n m. apply map_bsplice_comm. rewrite app_length. lia.
+Qed.
+
+
+(* substitution on bindings *)
+Definition bsubst i u (b: binding) : binding :=
+  match b with (is_ty, T) => (is_ty, subst T i u) end.
+
+(* position-dependent substitution of each entry in J'.
+   Entry b at depth k (with k entries below it in J') is substituted
+   with splice i k T1, because there are k bindings between it and the base env. *)
+Fixpoint msubst (J': list binding) (i: nat) (T1: tm) : list binding :=
+  match J' with
+  | [] => []
+  | b :: bs => bsubst i (splice i (length bs) T1) b :: msubst bs i T1
+  end.
+
+Lemma msubst_length: forall J' i T1,
+    length (msubst J' i T1) = length J'.
+Proof.
+  induction J'; intros; simpl; auto.
+Qed.
+
+(* key identity: substituting after a splice that created the variable cancels to a smaller splice *)
+Fixpoint subst_splice_cancel (e: tm) : forall n m u,
+    subst (splice n (S m) e) n u = splice n m e.
+Proof.
+  destruct e; intros; simpl;
+    try reflexivity;
+    try (rewrite ?subst_splice_cancel; reflexivity);
+    try (rewrite ?subst_splice_cancel; rewrite ?subst_splice_cancel; reflexivity);
+    (* TVar *)
+    try (bdestruct (i <? n); simpl;
+         [destruct (Nat.eq_dec i n); [lia|]; bdestruct (i <? n); [reflexivity|lia]
+         |destruct (Nat.eq_dec (i + S m) n); [lia|]; bdestruct (i + S m <? n); [lia|f_equal; lia]]).
+Defined.
+
+Lemma bsubst_bsplice_cancel: forall b i m u,
+    bsubst i u (bsplice i (S m) b) = bsplice i m b.
+Proof.
+  intros [b0 t]. intros. simpl. rewrite subst_splice_cancel. reflexivity.
+Qed.
+
+(* ---------- env extension lemmas  ---------- *)
+
+
+Lemma ext_length: forall b G,
+    length (ext b G) = S (length G).
+Proof.
+  intros. simpl. rewrite map_length. eauto.
+Qed.
+
+Lemma ext_unfold: forall b G,
+    ext b G = (bsplice (length G) 1 b) :: map (bsplice (length G) 1) G.
+Proof.
+  intros. unfold ext. simpl. eauto. 
+Qed.
+
+Lemma indexr_head_ext: forall b G,
+    indexr (length G) (ext b G) = Some (bsplice (length G) 1 b).
+Proof.
+  intros. 
+  unfold ext. remember (map _ _) as G'.
+  simpl in HeqG'. subst G'. remember (map _ _) as G''.
+  replace (length G) with (length G''). rewrite indexr_head. eauto.
+  subst G''. rewrite map_length. eauto.
+Qed.
+
+Check indexr_skip. 
+
+Lemma indexr_skip_ext: forall i b G,
+    i <> length G ->
+    indexr i (ext b G) = indexr i (map (bsplice (length G) 1) G).
+Proof.
+  intros. 
+  unfold ext. remember (map _ _) as G'.
+  simpl in HeqG'. subst G'. remember (map _ _) as G''.
+  rewrite indexr_skip. eauto.  
+  subst G''. rewrite map_length. eauto.
+Qed.
 
 (* ---------- other helper lemmas (semantics)  ---------- *)
 
@@ -453,7 +624,7 @@ Definition vt_all A (TF: A -> tpe): tpe :=
     | vtabs H ty =>
         forall T1,
           exists vy,
-            tevaln H ty vy /\
+            tevaln (vbool false::H) ty vy /\
             (TF T1) vy
     | _ => False
     end.
@@ -467,9 +638,97 @@ Fixpoint val_sort (K: tm) : Type :=
   | _ => unit
   end.
 
+Fixpoint val_sort1 (b: binding) : Type :=
+  match b with
+  | (false, _) => unit
+  | (true, K) => val_sort K
+  end.
+
+
+Fixpoint val_sort_splice (K: tm) : forall i n,
+    val_sort (splice i n K) = val_sort K.
+Proof.
+  destruct K; intros; simpl; try reflexivity.
+  - rewrite val_sort_splice, val_sort_splice. reflexivity.
+Defined.
+
+Lemma val_sort1_bsplice: forall b i n,
+    val_sort1 (bsplice i n b) = val_sort1 b.
+Proof.
+  intros [is_ty T] i n. destruct is_ty; simpl.
+  - rewrite val_sort_splice. reflexivity.
+  - reflexivity.
+Defined.
+
+Definition vs_cast {K} (i n: nat) (v: val_sort (splice i n K)) : val_sort K :=
+  eq_rect _ (fun T => T) v _ (val_sort_splice K i n).
+
+Definition vs_uncast {K} (i n: nat) (v: val_sort K) : val_sort (splice i n K) :=
+  eq_rect _ (fun T => T) v _ (eq_sym (val_sort_splice K i n)).
+
+Definition vs1_uncast {K} (i n: nat) (v: val_sort1 K) : val_sort1 (bsplice i n K) :=
+  eq_rect _ (fun T => T) v _ (eq_sym (val_sort1_bsplice K i n)).
+
+Lemma vs_cast_uncast: forall K i n (v: val_sort K),
+    vs_cast i n (vs_uncast i n v) = v.
+Proof.
+  intros. unfold vs_cast, vs_uncast.
+  generalize (val_sort_splice K i n).
+  intros e. destruct e. reflexivity.
+Defined.
+
+Lemma vs_uncast_cast: forall K i n (v: val_sort (splice i n K)),
+    vs_uncast i n (vs_cast i n v) = v.
+Proof.
+  intros. unfold vs_cast, vs_uncast.
+  generalize (val_sort_splice K i n).
+  intros e. destruct e. reflexivity.
+Defined.
+
+Lemma vs_uncast_fun: forall K1 K2 i n (f: val_sort K1 -> val_sort K2)
+    (x: val_sort (splice i n K1)),
+    (vs_uncast (K:=TFun K1 K2) i n f) x = vs_uncast i n (f (vs_cast i n x)).
+Proof.
+  intros. unfold vs_cast, vs_uncast.
+  simpl. unfold eq_sym, eq_ind_r, eq_rect, eq_ind.
+  generalize (val_sort_splice K1 i n).
+  generalize (val_sort_splice K2 i n).
+  intros e2 e1. destruct e1, e2. reflexivity.
+Defined.
+
+Lemma vs_cast_fun: forall K1 K2 i n (f: val_sort (splice i n K1) -> val_sort (splice i n K2))
+    (x: val_sort K1),
+    vs_cast i n (f (vs_uncast i n x)) = (vs_cast (K:=TFun K1 K2) i n f) x.
+Proof.
+  intros. unfold vs_cast, vs_uncast.
+  simpl. unfold eq_sym, eq_ind_r, eq_rect, eq_ind.
+  generalize (val_sort_splice K1 i n).
+  generalize (val_sort_splice K2 i n).
+  intros e2 e1. destruct e1, e2. reflexivity.
+Defined.
+
+Lemma vt_all_cast: forall K i n (F1: val_sort K -> tpe) (F2: val_sort (splice i n K) -> tpe),
+    (forall x, F1 x = F2 (vs_uncast i n x)) ->
+    vt_all (val_sort K) F1 = vt_all (val_sort (splice i n K)) F2.
+Proof.
+  intros K i n F1 F2 HF.
+  unfold vt_all. apply functional_extensionality. intros v.
+  destruct v; try reflexivity.
+  apply propositional_extensionality.
+  split; intros Hall.
+  - intros T1.
+    specialize (Hall (vs_cast i n T1)). destruct Hall as [vy [? ?]].
+    exists vy. split. auto.
+    pose proof (HF (vs_cast i n T1)) as E.
+    rewrite E in H0. rewrite (vs_uncast_cast K i n) in H0. exact H0.
+  - intros T1.
+    specialize (Hall (vs_uncast i n T1)). destruct Hall as [vy [? ?]].
+    exists vy. split. auto.
+    pose proof (HF T1) as E. rewrite E. exact H0.
+Defined.
 
 Definition env_kv J :=
-  forall x K, indexr x J = Some K -> val_sort K.
+  forall x b, indexr x J = Some b -> val_sort1 b.
 
 Lemma envkv_nil:
   env_kv nil.
@@ -477,10 +736,10 @@ Proof.
   intros ???. inversion H.
 Defined.
 
-Lemma envkv_cons: forall J K,
-    val_sort K ->
+Lemma envkv_cons: forall J b,
+    val_sort1 b ->
     env_kv J ->
-    env_kv (K::J).
+    env_kv (b::J).
 Proof.
   intros. intros ???.
   destruct (Nat.eq_dec x (length J)). subst.
@@ -488,25 +747,49 @@ Proof.
   rewrite indexr_skip in H. eapply X0. eauto. eauto.
 Defined.
 
-
-Require Import Coq.Arith.Compare_dec.
-
 Lemma indexr_hit: forall {T} J' J (K:T) ,
     indexr (length J) (J' ++ K :: J) = Some K.
 Proof.
   intros. rewrite indexr_skips. rewrite indexr_head. eauto. simpl. eauto.
 Qed.
 
-Lemma envkv_weaken: forall J' J K,
-    val_sort K ->
+Lemma envkv_weaken: forall J' J b,
+    val_sort1 b ->
     env_kv (J'++J) ->
-    env_kv (J'++K::J).
+    env_kv (J'++b::J).
 Proof.
   intros. intros ???.
   destruct (Nat.eq_dec x (length J)). subst.
   rewrite indexr_hit in H. inversion H. subst. eauto.
   rewrite indexr_splice2 in H; eauto.
 Defined.
+
+Lemma envkv_splice: forall i n J,
+    env_kv J ->
+    env_kv (map (bsplice i n) J).
+Proof.
+  intros. intros ???.
+  eapply indexr_map'' in H. destruct H. subst b.
+  eapply vs1_uncast. eapply X. eauto. 
+Defined.
+
+Lemma envkv_cons2: forall J b,
+    val_sort1 b ->
+    env_kv J ->
+    env_kv (map (bsplice (length J) 1) (b::J)).
+Proof.
+  intros. eapply envkv_splice. eapply envkv_cons. eauto. eauto. 
+Defined.
+
+Lemma envkv_weaken2: forall J' J b,
+    val_sort1 b ->
+    env_kv (J'++J) ->
+    env_kv (map (bsplice (length J) 1) (J'++b::J)).
+Proof.
+  intros. eapply envkv_splice. eapply envkv_weaken. eauto. eauto. 
+Defined.
+
+
 
 
 Fixpoint val_type {J T K} (h : has_kind J T K) (W : env_kv J) {struct h}: val_sort K :=
@@ -516,38 +799,38 @@ Fixpoint val_type {J T K} (h : has_kind J T K) (W : env_kv J) {struct h}: val_so
   | k_bool _, _, _ =>
       vt_bool
   | k_var _ x K IX, _, _ =>
-      W x K IX
+      W x (true, K) IX
   | k_fun _ T1 T2 h1 h2, _, _ =>
       vt_pi (val_type h1 W) (fun vx => val_type h2 W)
   | k_all _ K1 T2 h, _, _ =>
-      vt_all (val_sort K1) (fun VT1 => val_type h (envkv_cons _ _ VT1 W))
+      vt_all (val_sort K1) (fun VT1 => val_type h (envkv_cons2 _ _ (VT1 : val_sort1 (true, K1)) W))
   | k_karr _ _ _ K1 K2, _, _ =>
       tt
   | k_tabs _ K1 T2 K2 h, _, _ =>
-      (fun VT1 => val_type h (envkv_cons _ _ VT1 W))
+      (fun VT1 => val_type h (envkv_cons2 _ _ (VT1 : val_sort1 (true, K1)) W))
   | k_tapp _ TF TX K1 K2 hf hx, _, _ =>
       val_type hf W (val_type hx W)
   end.
 
 
 
-Definition exp_type H J (h2: env_kv J) t T :=
-  exists v (h1: has_kind J T TStar),
+Definition exp_type H G (h2: env_kv G) t T :=
+  exists v (h1: has_kind G T TStar),
     tevaln H t v /\
     val_type h1 h2 v.
 
-Definition env_type (H: venv) (G: tenv) (J: kenv) (h2: env_kv J):=
+Definition env_type (H: venv) (G: tenv) (h2: env_kv G):=
   length H = length G /\
   forall x T,
-    indexr x G = Some T ->
-    exists v (h1: has_kind J T TStar),
+    indexr x G = Some (false, T) ->
+    exists v (h1: has_kind G T TStar),
       indexr x H = Some v /\
       val_type h1 h2 v.
 
-Definition sem_type G J t T :=
-  forall H (h2: env_kv J),
-    env_type H G J h2 ->
-    exp_type H J h2 t T.
+Definition sem_type G t T :=
+  forall H (h2: env_kv G),
+    env_type H G h2 ->
+    exp_type H G h2 t T.
 
 
 (* ---------- LR helper lemmas  ---------- *)
@@ -564,7 +847,7 @@ Proof.
   induction a; intros K2' b; inversion b; subst; intros.
   - eauto.
   - eauto.
-  - congruence.
+  - unfold bind_ty in *. congruence.
   - eauto.
   - eauto.
   - eauto.
@@ -605,53 +888,102 @@ Proof.
 Qed.
 
 
+
 (* weakening *)
 
 Fixpoint haskind_weaken1 T: forall J' J K K1,
     has_kind (J' ++ J) T K ->
-    has_kind (J' ++ K1 :: J) (splice (length J) 1 T) K.
+    has_kind (map (bsplice (length J) 1) (J' ++ K1 :: J)) (splice (length J) 1 T) (splice (length J) 1 K).
 Proof.
   destruct T; intros; simpl in *.
   - (* TStar *) inversion H; subst. eapply k_star.
   - (* TBox *) inversion H.
   - (* TBool *) inversion H; subst. eapply k_bool.
-  - (* TVar *) inversion H; subst. eapply k_var. replace (i+1) with (1+i). 2: lia.
-    erewrite indexr_splice1. eauto.
-  - (* TFun *) inversion H; subst. eapply k_fun. eauto. eauto.
-    (* TKArr *) eapply k_karr. eauto. eauto. 
-  - (* TAll *) inversion H; subst. eapply k_all. eapply haskind_weaken1 with (J':=T1::J'). eauto.
-  - (* TTAbs *) inversion H; subst. 
-  - (* TTApp *) inversion H; subst. 
+  - (* TFun *) inversion H; subst.
+    + eapply k_fun.
+      eapply (haskind_weaken1 T1 J' J TStar K1 H2).
+      eapply (haskind_weaken1 T2 J' J TStar K1 H4).
+    + eapply k_karr. 
+      eapply (haskind_weaken1 T1 J' J TBox K1 H2).
+      eapply (haskind_weaken1 T2 J' J TBox K1 H4).
+  - (* TAll *) inversion H; subst. eapply k_all.
+    (* H3: has_kind (ext (bind_ty T1) (J'++J)) T2 TStar *)
+    unfold ext in H3.
+    replace (bind_ty T1 :: J' ++ J) with ((bind_ty T1 :: J') ++ J) in H3 by reflexivity.
+    rewrite map_app in H3.
+    eapply haskind_weaken1 with (K1 := bsplice (length (J'++J)) 1 K1) in H3.
+    rewrite map_length in H3.
+    (* Reassemble inner list *)
+    change (bsplice (length (J' ++ J)) 1 K1 :: map (bsplice (length (J' ++ J)) 1) J)
+      with (map (bsplice (length (J' ++ J)) 1) (K1 :: J)) in H3.
+    rewrite <- map_app in H3. simpl app in H3.
+    (* H3: has_kind (map (bsplice (length J) 1) (map (bsplice (length (J'++J)) 1) (bind_ty T1 :: J' ++ K1 :: J)))
+                     (splice (length J) 1 T2) TStar *)
+    (* Use weaken_ext_comm to commute the double map *)
+    rewrite weaken_ext_comm in H3.
+    (* Now match the goal *)
+    unfold ext.
+    change (bind_ty (splice (length J) 1 T1)) with (bsplice (length J) 1 (bind_ty T1)).
+    change (bsplice (length J) 1 (bind_ty T1) :: map (bsplice (length J) 1) (J' ++ K1 :: J))
+      with (map (bsplice (length J) 1) (bind_ty T1 :: J' ++ K1 :: J)).
+    rewrite map_length, app_length. simpl length.
+    rewrite app_length in H3.
+    replace (length J' + S (length J)) with (length J' + length J + 1) by lia.
+    eapply H3.
   - inversion H.
   - inversion H.
+  - (* TVar *) inversion H; subst. eapply k_var.
+    replace (i + 1) with (S i) by lia.
+    erewrite indexr_map. (* with (v := Some (true, K)). *)
+    2: { erewrite indexr_splice1. eauto. }
+    simpl. reflexivity.
   - inversion H.
-  - (* TTApp *) inversion H; subst. eapply k_tapp. eauto. eauto.
-  - (* TTAbs *) inversion H; subst. eapply k_tabs. eapply haskind_weaken1 with (J':=T1::J'). eauto.
+  - inversion H.
+  - (* TTApp *) inversion H; subst; simpl.
+    exact (k_tapp _ _ _ _ _ (haskind_weaken1 T1 J' J _ K1 H2) (haskind_weaken1 T2 J' J _ K1 H4)).
+  - (* TTAbs *) inversion H; subst. eapply k_tabs.
+    unfold ext in H3.
+    replace (bind_ty T1 :: J' ++ J) with ((bind_ty T1 :: J') ++ J) in H3 by reflexivity.
+    rewrite map_app in H3.
+    eapply haskind_weaken1 with (K1 := bsplice (length (J'++J)) 1 K1) in H3.
+    rewrite map_length in H3.
+    change (bsplice (length (J' ++ J)) 1 K1 :: map (bsplice (length (J' ++ J)) 1) J)
+      with (map (bsplice (length (J' ++ J)) 1) (K1 :: J)) in H3.
+    rewrite <- map_app in H3. simpl app in H3.
+    rewrite weaken_ext_comm in H3.
+    unfold ext.
+    change (bind_ty (splice (length J) 1 T1)) with (bsplice (length J) 1 (bind_ty T1)).
+    change (bsplice (length J) 1 (bind_ty T1) :: map (bsplice (length J) 1) (J' ++ K1 :: J))
+      with (map (bsplice (length J) 1) (bind_ty T1 :: J' ++ K1 :: J)).
+    rewrite map_length, app_length. simpl length.
+    rewrite app_length in H3.
+    replace (length J' + S (length J)) with (length J' + length J + 1) by lia.
+    eapply H3.
 Defined.
 
 
 Lemma haskind_extend: forall T J K K1,
     has_kind J T K ->
-    has_kind (K1 :: J) (splice (length J) 1 T) K.
+    has_kind (ext K1 J) (splice (length J) 1 T) (splice (length J) 1 K).
 Proof.
-  intros. eapply haskind_weaken1 with (J':=[]). eauto.
+  intros. unfold ext. eapply haskind_weaken1 with (J':=[]). eauto.
 Defined.
 
 Fixpoint haskind_extend_mult J': forall T J K,
     has_kind J T K ->
-    has_kind (J'++ J) (splice (length J) (length J') T) K.
+    has_kind (mext J' J) (splice (length J) (length J') T) (splice (length J) (length J') K).
 Proof.
   destruct J'; intros; simpl in *.
-  - rewrite splice_zero. eapply H.
+  - rewrite !splice_zero. eapply H.
   - eapply haskind_extend_mult in H. eapply haskind_extend in H.
-    rewrite app_length in H. rewrite splice_acc' in H. eapply H.
+    rewrite mext_length in H. rewrite !splice_acc' in H. eapply H.
 Defined.
 
 Lemma aux0: forall i i' J K
   (eq: i = i')
-  (h2: forall i K, indexr i (J) = Some K -> val_sort K)
-  (h2A: indexr i (J) = Some K -> val_sort K)
-  (h2B: indexr i' (J) = Some K -> val_sort K)
+  (h2: forall i K, indexr i J = Some K -> val_sort1 K)
+  (h2A: indexr i J = Some K -> val_sort1 K)
+  (h2B: indexr i' J = Some K -> val_sort1 K)
   (eq2A: h2A = h2 i K)
   (eq2B: h2B = h2 i' K)
   eA eB,
@@ -671,7 +1003,7 @@ Proof.
     remember indexr_head. replace IX with e. 2: eapply proof_irrelevance.
     cbn.
     remember (eq_ind (if length J =? length J then Some K1 else indexr (length J) J)
-      (fun o : option tm => o = Some K1) e (Some K1) e).
+      (fun o : option binding => o = Some K1) e (Some K1) e).
     simpl in e0.
     dependent destruction e0.
     cbn. eauto.
@@ -689,6 +1021,25 @@ Proof.
   - eapply aux0. eauto. eauto. eauto.
 Qed.
 
+Lemma envkv_cons2_head: forall J K1 vk h2 IX,
+    envkv_cons2 J K1 vk h2 (length J) K1 IX ~= (vs1_uncast (length J) 1 vk).
+Proof.
+  intros J K1 vk h2 IX.
+  unfold envkv_cons2. unfold envkv_splice.
+  remember (indexr_map'' _ _ _ _ _). destruct s.
+  remember (envkv_cons _ _ _ _ _ _ _). 
+  symmetry in Heqv. 
+  (* want to use envkv_cons_head *)
+Admitted.
+
+Lemma envkv_cons2_skip: forall J K1 K i vk (h2:env_kv J) IX IX',
+    i < length J ->
+    envkv_cons2 J K1 vk h2 i K IX' = h2 i K IX. (* ??? *)
+Proof.
+  intros.
+  unfold envkv_cons2. unfold envkv_splice. 
+Admitted. 
+
 
 Lemma envkv_weaken_hit: forall J' J K1 vk h2 IX,
     envkv_weaken J' J K1 vk h2 (length J) K1 IX = vk.
@@ -700,7 +1051,7 @@ Proof.
     remember (indexr_hit J' J K1). replace IX with e. 2: eapply proof_irrelevance.
     cbn.
     remember (eq_ind (indexr (length J) (J' ++ K1 :: J))
-      (fun o : option tm => o = Some K1) e (Some K1) e).
+      (fun o : option binding => o = Some K1) e (Some K1) e).
     simpl in e0.
     dependent destruction e0.
     cbn. eauto.
@@ -828,95 +1179,107 @@ Proof.
     Unshelve. simpl. eauto.
 Qed.
 
-Lemma valt_weaken: forall T J' J K1 K vk (h1: has_kind (J'++J) T K) h2,
-    val_type h1 h2 =
-    val_type (haskind_weaken1 T J' J K K1 h1)
-    (envkv_weaken J' J K1 vk h2).
+Lemma envkv_weaken_eq_extend2: forall J K1 vk h2,
+    envkv_weaken2 [] J K1 vk h2 = envkv_cons2 J K1 vk h2.
+Proof.
+  intros.
+  eapply functional_extensionality_dep. intros i.
+  eapply functional_extensionality_dep. intros K.
+  eapply functional_extensionality_dep. intros IX.
+  simpl in *.
+  assert ((if i =? length (map (bsplice (length J) 1) J)
+        then Some (bsplice (length J) 1 K1)
+        else indexr i (map (bsplice (length J) 1) J)) = Some K). eapply IX.
+  bdestruct (i =? length (map (bsplice (length J) 1) J)).
+  - inversion H. subst.
+    admit. 
+  - admit.
+Admitted.
+
+(* TODO: valt_weaken, valt_extend, valt_extend' need updating for ext-based environments.
+   Commented out temporarily to focus on syntactic lemmas first. *)
+(*
+Lemma valt_weaken: ...
+Lemma valt_extend: ...
+Lemma valt_extend': ...
+*)
+
+Lemma valt_weaken: forall T J' J K1 K vk (h1: has_kind (app J' J) T K) h2,
+      val_type h1 h2 ~=
+      val_type (haskind_weaken1 T J' J _ K1 h1)
+         (envkv_weaken2 J' J K1 vk h2).
 Proof.
   intros T. induction T; intros; simpl in *.
-  - (* TStar *)
-    dependent destruction h1.
-    simpl. eauto.
-  - (* TBox *)
-    inversion h1.
-  - (* TBool *)
-    dependent destruction h1.
-    simpl. split; eauto.
-  - (* TVar *)
-    dependent destruction h1.
-    remember (k_var (J'++J) i K e) as hx1.
-    remember ((haskind_weaken1 (TVar i) J' J K K1 hx1)) as hx1'.
-    remember ((envkv_weaken J' J K1 vk h2)) as h2'.
-    dependent destruction hx1. inversion Heqhx1. rewrite Heqhx1 in *.
-    dependent destruction hx1'.
-    simpl.
-    subst h2'. eapply aux1.
-  - (* TFun *)
-    dependent destruction h1.
-    + simpl in *.
-    assert (val_type h1_1 h2 = val_type (haskind_weaken1 T1 J' J TStar K1 h1_1) (envkv_weaken J' J K1 vk h2)). eapply IHT1.
-    assert (val_type h1_2 h2 = val_type (haskind_weaken1 T2 J' J TStar K1 h1_2) (envkv_weaken J' J K1 vk h2)). eapply IHT2.
-    rewrite H, H0. eauto.
-    + (* TKArr *)
-    simpl. eauto.
-  - (* TAll *)
-    dependent destruction h1. simpl.
-    assert (forall VT1, val_type h1 (envkv_cons (J'++J) T1 VT1 h2) =
-                          val_type (haskind_weaken1 T2 (T1::J') J TStar K1 h1) (envkv_weaken (T1::J') J K1 vk (envkv_cons (J'++J) T1 VT1 h2))). {
-    intros.
-    specialize IHT2 with (J':=T1::J') (J:=J) (vk:=vk) (h1:=h1) (h2:=(envkv_cons (J'++J) T1 VT1 h2)).
-    eapply IHT2. }
-    eapply functional_extensionality in H.
-    rewrite H.
-    assert (forall VT1,
-     val_type (haskind_weaken1 T2 (T1 :: J') J TStar K1 h1) (envkv_weaken (T1 :: J') J K1 vk (envkv_cons (J' ++ J) T1 VT1 h2)) = val_type (haskind_weaken1 T2 (T1 :: J') J TStar K1 h1) (envkv_cons (J' ++ K1 :: J) T1 VT1 (envkv_weaken J' J K1 vk h2))).
-    intros. rewrite aux2. eauto.
-    eapply functional_extensionality in H0.
-    rewrite H0. eauto.
-  - inversion h1. (* TKArr *)
-  - inversion h1. (* TTAbs *)
-  - inversion h1. (* TTApp *)
+  - dependent destruction h1. reflexivity.
   - inversion h1.
-  - inversion h1. 
-  - (* TTApp *)
-    dependent destruction h1. simpl.
-    specialize (IHT1) with (h1:=h1_1) (h2:=h2).
-    erewrite IHT1.
-    specialize (IHT2) with (h1:=h1_2) (h2:=h2).
-    erewrite IHT2.
-    eauto.
-  - (* TTAbs *)
-    dependent destruction h1.
+  - dependent destruction h1. reflexivity.
+  - dependent destruction h1.
+    + simpl.
+      rewrite (IHT1 J' J K1 TStar vk h1_1 h2).
+      rewrite (IHT2 J' J K1 TStar vk h1_2 h2).
+      reflexivity.
+    + simpl. reflexivity.
+  - dependent destruction h1. simpl.
+    admit. (* f_equal.
+    apply functional_extensionality. intros VT1.
+    specialize (IHT2 (bind_ty T1 :: J') J K1 TStar vk h1
+      (envkv_cons (J' ++ J) (bind_ty T1) (VT1 : val_sort1 (bind_ty T1)) h2)).
+    rewrite aux2. exact IHT2. *)
+  - inversion h1.
+  - inversion h1.
+  - dependent destruction h1.
+    remember (k_var (J' ++ J) i K e) as hx1.
+    remember (haskind_weaken1 (TVar i) J' J K K1 hx1) as hx1'.
+    remember (envkv_weaken J' J K1 vk h2) as h2'.
+    dependent destruction hx1. inversion Heqhx1. rewrite Heqhx1 in *.
+    dependent destruction hx1'. simpl.
+    subst h2'.
+    admit. (* match goal with
+    | |- _ = envkv_weaken _ _ _ _ _ _ _ ?pf =>
+        replace pf with e1 by apply proof_irrelevance
+    end.
+    exact (aux1 J' J h2 i (bind_ty K) e K1 vk e1).*)
+  - inversion h1.
+  - inversion h1.
+  - dependent destruction h1. simpl.
+    admit. (*
+    rewrite (IHT1 J' J K1 _ vk h1_1 h2).
+    rewrite (IHT2 J' J K1 _ vk h1_2 h2).
+    reflexivity. *)
+  - dependent destruction h1.
     remember (k_tabs (J' ++ J) T1 T2 K2 h1) as h1'.
     dependent destruction h1'.
     replace h1 with h1' in * by (eapply hk_unique).
-    simpl in *. eapply functional_extensionality.
-    intros.
-    specialize IHT2 with (J':=T1::J') (h1:=h1') (h2:=(envkv_cons (J' ++ J) T1 x h2)) (vk:=vk).
-    rewrite aux2. eapply IHT2. 
-Qed.
+    simpl.
+    admit. (*
+    apply functional_extensionality. intros VT1.
+    specialize (IHT2 (bind_ty T1 :: J') J K1 K2 vk h1'
+      (envkv_cons (J' ++ J) (bind_ty T1) (VT1 : val_sort1 (bind_ty T1)) h2)).
+    rewrite aux2. exact IHT2. *)
+Admitted.
 
 
 Lemma valt_extend: forall T J K1 vk (h1: has_kind J T TStar) h2 v2,
     val_type h1 h2 v2 <->
     val_type (haskind_extend T J TStar K1 h1)
-    (envkv_cons J K1 vk h2) v2.
-Proof.
+    (envkv_cons2 J K1 vk h2) v2.
+Proof. 
   intros.
   specialize valt_weaken with (J':=[]). simpl. intros. unfold haskind_extend.
-  replace (envkv_cons J K1 vk h2) with (envkv_weaken [] J K1 vk h2).
-  erewrite H. 2: eapply envkv_weaken_eq_extend. split; eauto.
+  specialize (H _ _ _ _ vk h1 h2). rewrite H. 
+  rewrite envkv_weaken_eq_extend2. split; eauto.
 Qed.
 
+
 Lemma valt_extend': forall T J K1 K vk (h1: has_kind J T K) h2,
-    val_type h1 h2 =
+    val_type h1 h2 ~=
     val_type (haskind_extend T J K K1 h1)
-    (envkv_cons J K1 vk h2).
+    (envkv_cons2 J K1 vk h2).
 Proof.
   intros.
   specialize valt_weaken with (J':=[]). simpl. intros. unfold haskind_extend.
-  replace (envkv_cons J K1 vk h2) with (envkv_weaken [] J K1 vk h2).
-  erewrite H. 2: eapply envkv_weaken_eq_extend. split; eauto.
+  replace (envkv_cons2 J K1 vk h2) with (envkv_weaken2 [] J K1 vk h2).
+  erewrite H. 2: eapply envkv_weaken_eq_extend2. split; eauto.
 Qed.
 
 
@@ -945,55 +1308,91 @@ Proof.
 Defined.
 
 
+(*
 Fixpoint hask_subst T2: forall J' J T1 K1 K2,
-    has_kind (J' ++ K1 :: J) T2 K2 ->
+    has_kind (mext J' (ext (bind_ty K1) J)) T2 K2 ->
     has_kind J T1 K1 ->
-    has_kind (J'++J) (subst T2 (length J) (splice (length J) (length J') T1)) K2.
+    has_kind (mext (msubst J' (length J) T1) J)
+             (subst T2 (length J) (splice (length J) (length J') T1))
+             (subst K2 (length J) (splice (length J) (length J') T1)).
 Proof.
-  destruct T2; intros; simpl in *.
-  - (* TStar *) inversion H; subst. eapply k_star.
-  - (* TBox *) inversion H.
-  - (* TBool *) inversion H; subst. eapply k_bool.
+  destruct T2; intros J' J T1 K1 K2 HK HT1.
+  - (* TStar *) simpl in *. inversion HK; subst. simpl. eapply k_star.
+  - (* TBox *) inversion HK.
+  - (* TBool *) simpl in *. inversion HK; subst. simpl. eapply k_bool.
+  - (* TFun *) simpl in *. inversion HK; subst; simpl.
+    + eapply k_fun. 
+      eapply (hask_subst T2_1 J' J T1 K1 TStar H1 HT1).
+      eapply (hask_subst T2_2 J' J T1 K1 TStar H3 HT1).
+    + eapply k_karr.
+      eapply (hask_subst T2_1 J' J T1 K1 TBox H1 HT1).
+      eapply (hask_subst T2_2 J' J T1 K1 TBox H3 HT1).
+  - (* TAll *) simpl in *. inversion HK; subst. simpl. eapply k_all. rewrite splice_acc.
+    change (ext (bind_ty (subst T2_1 (length J) (splice (length J) (length J') T1)))
+                (mext (msubst J' (length J) T1) J))
+      with (mext (msubst (bind_ty T2_1 :: J') (length J) T1) J).
+    eapply hask_subst with (J':=bind_ty T2_1::J') (K2:=TStar); eauto.
+  - inversion HK.
+  - inversion HK.
   - (* TVar *)
-    inversion H; subst.
+    inversion HK; subst.
     destruct (Nat.eq_dec i (length J)) as [Heq | Hneq].
-    + eapply haskind_extend_mult. eapply xxx4. eauto. eapply xxx3; eauto.
-    + eapply k_var.
-      rewrite indexr_splice2 in H2. eapply H2. eauto.
-  - (* TFun *) inversion H; subst.
-    + eapply k_fun. eauto. eauto.
-    + (* TKArr *) eapply k_karr. eauto. eauto. 
-  - (* TAll *) inversion H; subst. eapply k_all. rewrite splice_acc.
-    eapply hask_subst with (J':=T2_1::J'). eauto. eauto.
-  - (* TKArr *) inversion H; subst. (* eapply k_karr. eauto. eauto. *)
-  - (* TTAbs *) inversion H; subst. (*eapply k_tabs. rewrite splice_acc.
-    eapply hask_subst with (J':=T2_1::J'). eauto. eauto.*)
-  - inversion H. 
-  - inversion H. 
-  - inversion H. 
-  - (* TTApp *) inversion H; subst. eapply k_tapp. eauto. eauto.
-  - (* TTAbs *) inversion H; subst. eapply k_tabs. rewrite splice_acc.
-    eapply hask_subst with (J':=T2_1::J'). eauto. eauto.
-Defined.
+    + (* i = n: substitute *)
+      subst i.
+      assert (HIX := indexr_mext_ext_hit J' J K1).
+      cbv zeta in HIX.
+      change (@indexr (prod bool tm)) with (@indexr binding) in H0.
+      rewrite HIX in H0. inversion H0; subst.
+      simpl.
+      destruct (Nat.eq_dec (length J) (length J)); [| congruence].
+      rewrite subst_splice_cancel.
+      eapply haskind_extend_mult_msubst; eauto.
+    + (* i <> n: shift *)
+      simpl.
+      destruct (Nat.eq_dec i (length J)); [congruence |].
+      change (@indexr (prod bool tm)) with (@indexr binding) in H0.
+      pose proof (indexr_mext_ext_subst J' J T1 K1 i K2 Hneq H0 HT1 HFC) as HIX.
+      cbv zeta in HIX.
+      eapply k_var. exact HIX.
+  - inversion HK.
+  - inversion HK.
+  - (* TTApp *) simpl in *. inversion HK; subst. simpl.
+    exact (k_tapp _ _ _ _ _ (hask_subst T2_1 J' J T1 K1 (TFun K0 K2) H1 HT1 HFC)
+                            (hask_subst T2_2 J' J T1 K1 K0 H3 HT1 HFC)).
+  - (* TTAbs *) simpl in *. inversion HK; subst. simpl.
+    eapply k_tabs. rewrite splice_acc.
+
+    change (ext (bind_ty (subst T2_1 (length J) (splice (length J) (length J') T1)))
+                (mext (msubst J' (length J) T1) J))
+      with (mext (msubst (bind_ty T2_1 :: J') (length J) T1) J).
+    (* IH: subst K3 n (splice n (S m) T1). Goal: subst K3 n (splice n m T1).
+       Both = K3 when fclosed K3 (length J). *)
+    assert (HFC3: fclosed K3 (length J)). admit.
+    pose proof (hask_subst T2_2 (bind_ty T2_1::J') J T1 K1 K3 H2 HT1 HFC) as IH.
+    simpl length in IH.
+    rewrite (subst_fclosed K3 (length J) (length J) (splice (length J) (S (length J')) T1) HFC3 (Nat.le_refl _)) in IH.
+    rewrite (subst_fclosed K3 (length J) (length J) (splice (length J) (length J') T1) HFC3 (Nat.le_refl _)).
+    exact IH.
+Admitted.*)
 
 Lemma hask_subst1: forall J T2 T1 K1,
-    has_kind (K1 :: J) T2 TStar ->
+    has_kind (ext (bind_ty K1) J) T2 TStar ->
     has_kind J T1 K1 ->
     has_kind J (subst T2 (length J) T1) TStar.
-Proof.
+Proof. (*
   intros. eapply hask_subst with (J':=[]) in H0.
   simpl in H0. rewrite splice_zero in H0. eauto.
-  simpl. eauto.
-Defined.
+  simpl. eauto. eauto. *)
+Admitted.
 
 Lemma hask_subst1': forall J T2 T1 K1 K,
-    has_kind (K1 :: J) T2 K ->
+    has_kind (ext (bind_ty K1) J) T2 K ->
     has_kind J T1 K1 ->
-    has_kind J (subst T2 (length J) T1) K.
-Proof.
+    has_kind J (subst T2 (length J) T1) (subst K (length J) T1).
+Proof. (*
   intros. apply hask_subst with (J':=[]) (T2:=T2) (K2:=K) in H0; auto.
-  simpl in H0. rewrite splice_zero in H0; auto.
-Defined.
+  simpl in H0. rewrite splice_zero in H0; auto. *)
+Admitted.
 
 
 Lemma aux1b'': forall J' J K1 K T1K WFJ i e0 e1,
@@ -1006,103 +1405,106 @@ Proof.
   erewrite envkv_weaken_ge. eauto. lia. lia.
 Qed.
 
-Lemma valt_subst: forall T2 J' J K1 K2 T1K WFJ T1 (h1f : has_kind (J'++K1 :: J) T2 K2) HK1,
+(* TODO: valt_subst and all downstream LR lemmas need ext-based updating.
+   Commented out to focus on syntactic hask_subst first. *)
+(*
     T1K = val_type (haskind_extend_mult J' T1 J K1 HK1) WFJ ->
-    val_type h1f (envkv_weaken J' J K1 T1K WFJ) =
+    val_type h1f (envkv_weaken J' J (bind_ty K1) T1K WFJ) =
     val_type (hask_subst T2 J' J T1 K1 K2 h1f HK1) WFJ.
 Proof.
   intros T2. induction T2; intros; simpl in *.
   - (* TStar *) dependent destruction h1f. simpl. eauto.
   - (* TBox *) inversion h1f.
   - (* TBool *) dependent destruction h1f. simpl. eauto.
-  - (* TVar *)
-    dependent destruction h1f.
-    remember (k_var (J' ++ K1 :: J) i K e) as hx1.
-    remember (hask_subst (TVar i) J' J T1 K1 K hx1 HK1) as hx1'.
-    remember (envkv_weaken J' J K1 T1K WFJ) as h2'.
-    dependent destruction hx1. simpl.
-
-    simpl in *. remember (Nat.eq_dec i (length J)).
-    destruct s.
-    + subst i.
-      simpl in *.
-      assert (HK1EQ: K1 = K). eapply xxx3; eauto.
-      subst K1.
-      (* Goal: val_type hx1 h2' = val_type hx1' WFJ
-         where hx1 is (k_var ... e0), h2' = envkv_weaken ...,
-         and hx1' = hask_subst (TVar (length J)) ... *)
-      subst h2'.
-      simpl. rewrite envkv_weaken_hit.
-      subst T1K.
-      (* Goal: val_type (haskind_extend_mult ...) WFJ = val_type hx1' WFJ *)
-      f_equal. eapply hk_unique.
-
-    + dependent destruction hx1'.
-      simpl. subst h2'. eapply aux1b''. eauto.
-
-  - (*TFun*) dependent destruction h1f; simpl.
-    + assert (H21: val_type h1f1 (envkv_weaken J' J K1 T1K WFJ) = val_type (hask_subst T2_1 J' J T1 K1 TStar h1f1 HK1) WFJ). apply IHT2_1. auto. rewrite H21.
-    assert (H22: val_type h1f2 (envkv_weaken J' J K1 T1K WFJ) = val_type (hask_subst T2_2 J' J T1 K1 TStar h1f2 HK1) WFJ). apply IHT2_2. auto. rewrite H22. auto.
-    + (*TKArr*) eauto. 
-  - (*TAll*) dependent destruction h1f. simpl.
-    assert (HVT: forall VT1, val_type (haskind_extend_mult (T2_1 :: J') T1 J K1 HK1) (envkv_cons (J' ++ J) T2_1 VT1 WFJ) = val_type (haskind_extend_mult J' T1 J K1 HK1) WFJ). { intros.
+  - (* TFun *) dependent destruction h1f; simpl.
+    + assert (H21: val_type h1f1 (envkv_weaken J' J (bind_ty K1) T1K WFJ) = val_type (hask_subst T2_1 J' J T1 K1 TStar h1f1 HK1) WFJ). apply IHT2_1. auto. rewrite H21.
+      assert (H22: val_type h1f2 (envkv_weaken J' J (bind_ty K1) T1K WFJ) = val_type (hask_subst T2_2 J' J T1 K1 TStar h1f2 HK1) WFJ). apply IHT2_2. auto. rewrite H22. auto.
+    + (* TKArr *) eauto.
+  - (* TAll *) dependent destruction h1f. simpl.
+    assert (HVT: forall VT1, val_type (haskind_extend_mult (bind_ty T2_1 :: J') T1 J K1 HK1) (envkv_cons (J' ++ J) (bind_ty T2_1) VT1 WFJ) = val_type (haskind_extend_mult J' T1 J K1 HK1) WFJ). { intros.
       simpl. elim_eq_rect. simpl. elim_eq_rect. simpl.
       rewrite <- valt_extend'. reflexivity.
     }
-    assert (HV: forall VT1, val_type h1f (envkv_cons (J' ++ K1 :: J) T2_1 VT1 (envkv_weaken J' J K1 T1K WFJ)) =
-      val_type (eq_rec_r (fun t : tm => has_kind (T2_1 :: J' ++ J) (subst T2_2 (length J) t) TStar) (hask_subst T2_2 (T2_1 :: J') J T1 K1 TStar h1f HK1) (splice_acc T1 (length J) (length J') 1))
-      (envkv_cons (J' ++ J) T2_1 VT1 WFJ)). { intros.
+    assert (HV: forall VT1, val_type h1f (envkv_cons (J' ++ bind_ty K1 :: J) (bind_ty T2_1) VT1 (envkv_weaken J' J (bind_ty K1) T1K WFJ)) =
+      val_type (eq_rec_r (fun t : tm => has_kind (bind_ty T2_1 :: J' ++ J) (subst T2_2 (length J) t) TStar) (hask_subst T2_2 (bind_ty T2_1 :: J') J T1 K1 TStar h1f HK1) (splice_acc T1 (length J) (length J') 1))
+      (envkv_cons (J' ++ J) (bind_ty T2_1) VT1 WFJ)). { intros.
       rewrite splice_acc. rewrite aux2.
-      specialize (IHT2_2 (T2_1 :: J') J K1 TStar T1K (envkv_cons (J' ++ J) T2_1 VT1 WFJ) T1 h1f HK1).
+      specialize (IHT2_2 (bind_ty T2_1 :: J') J K1 TStar T1K (envkv_cons (J' ++ J) (bind_ty T2_1) VT1 WFJ) T1 h1f HK1).
       specialize (HVT VT1). rewrite <- HVT in H.
       specialize (IHT2_2 H). auto.
     }
-    eapply functional_extensionality in HV. rewrite HV. auto.
-  - inversion h1f. (*TKArr*) 
+    f_equal.
+    apply functional_extensionality_dep. intro VT1.
+    exact (HV VT1).
   - inversion h1f.
   - inversion h1f.
+  - (* TVar *)
+    dependent destruction h1f.
+    remember (k_var (J' ++ bind_ty K1 :: J) i K e) as hx1.
+    remember (hask_subst (TVar i) J' J T1 K1 K hx1 HK1) as hx1'.
+    remember (envkv_weaken J' J (bind_ty K1) T1K WFJ) as h2'.
+    dependent destruction hx1. simpl.
+    simpl in *. remember (Nat.eq_dec i (length J)) as s.
+    destruct s.
+    + subst i.
+      simpl in *.
+      assert (HK1EQ': bind_ty K1 = bind_ty K). eapply xxx3; eauto.
+      assert (HK1EQ: K1 = K). inversion HK1EQ'. reflexivity.
+      subst K1.
+      subst h2'.
+      simpl. rewrite envkv_weaken_hit.
+      subst T1K.
+      f_equal. eapply hk_unique.
+    + dependent destruction hx1'.
+      simpl. subst h2'.
+      match goal with
+      | |- _ = WFJ _ _ ?pf =>
+          replace pf with e1 by apply proof_irrelevance
+      end.
+      exact (aux1b'' J' J (bind_ty K1) (bind_ty K) T1K WFJ i e0 e1 n).
   - inversion h1f.
   - inversion h1f.
-  - (*TTApp*) dependent destruction h1f. simpl.
+  - (* TTApp *) dependent destruction h1f. simpl.
     specialize (IHT2_2) with (h1f := h1f2). specialize (IHT2_2 T1K WFJ T1 HK1 H). rewrite IHT2_2.
     remember ((val_type (hask_subst T2_2 J' J T1 K1 K0 h1f2 HK1) WFJ)) as VT2.
     specialize (IHT2_1) with (h1f := h1f1). specialize (IHT2_1 T1K WFJ T1 HK1 H). rewrite IHT2_1. auto.
-  - (*TTAbs*) dependent destruction h1f. remember (k_tabs (J' ++ K1 :: J) T2_1 T2_2 K2 h1f) as h1f'.
+  - (* TTAbs *) dependent destruction h1f. remember (k_tabs (J' ++ bind_ty K1 :: J) T2_1 T2_2 K2 h1f) as h1f'.
     dependent destruction h1f'.
     replace h1f with h1f' in * by (eapply hk_unique).
     simpl. rewrite splice_acc.
     apply functional_extensionality. intro vk.
     rewrite aux2.
-    assert (HT1K: val_type (haskind_extend_mult (T2_1 :: J') T1 J K1 HK1) (envkv_cons (J' ++ J) T2_1 vk WFJ) = val_type (haskind_extend_mult J' T1 J K1 HK1) WFJ). { intros.
+    assert (HT1K: val_type (haskind_extend_mult (bind_ty T2_1 :: J') T1 J K1 HK1) (envkv_cons (J' ++ J) (bind_ty T2_1) vk WFJ) = val_type (haskind_extend_mult J' T1 J K1 HK1) WFJ). { intros.
       simpl. elim_eq_rect. simpl. elim_eq_rect. simpl.
       rewrite <- valt_extend'. reflexivity.
     } rewrite <- HT1K in H.
-    specialize (IHT2_2 (T2_1 :: J')) with (h1f := h1f') (WFJ := (envkv_cons (J' ++ J) T2_1 vk WFJ)) (T1K := T1K). specialize (IHT2_2 T1 HK1 H).
-    replace (val_type h1f' (envkv_weaken (T2_1 :: J') J K1 T1K (envkv_cons (J' ++ J) T2_1 vk WFJ))) with (val_type (hask_subst T2_2 (T2_1 :: J') J T1 K1 K2 h1f' HK1) (envkv_cons (J' ++ J) T2_1 vk WFJ)). (*using IHT2_2*)
+    specialize (IHT2_2 (bind_ty T2_1 :: J')) with (h1f := h1f') (WFJ := (envkv_cons (J' ++ J) (bind_ty T2_1) vk WFJ)) (T1K := T1K). specialize (IHT2_2 T1 HK1 H).
+    replace (val_type h1f' (envkv_weaken (bind_ty T2_1 :: J') J (bind_ty K1) T1K (envkv_cons (J' ++ J) (bind_ty T2_1) vk WFJ))) with (val_type (hask_subst T2_2 (bind_ty T2_1 :: J') J T1 K1 K2 h1f' HK1) (envkv_cons (J' ++ J) (bind_ty T2_1) vk WFJ)). (*using IHT2_2*)
     auto.
 Qed.
+*)
 
-
-Lemma valt_subst1: forall T2 J K1 T1K WFJ T1 (h1f : has_kind (K1 :: J) T2 TStar) HK1 vy,
+Lemma valt_subst1: forall T2 J K1 T1K WFJ T1 (h1f : has_kind (ext (bind_ty K1) J) T2 TStar) HK1 vy,
   T1K = val_type HK1 WFJ ->
-  val_type h1f (envkv_cons J K1 T1K WFJ) vy =
+  val_type h1f (envkv_cons2 J (bind_ty K1) T1K WFJ) vy =
   val_type (hask_subst1 J T2 T1 K1 h1f HK1) WFJ vy.
-Proof.
+Proof. (*
   intros.
   specialize valt_subst with (J':=[]). simpl. intros. unfold hask_subst1.
   unfold eq_rect. remember (splice_zero T1 (length J)).
   clear Heqe.
   dependent destruction e.
-  replace (envkv_cons J K1 T1K WFJ) with (envkv_weaken [] J K1 T1K WFJ).
+  replace (envkv_cons J (bind_ty K1) T1K WFJ) with (envkv_weaken [] J (bind_ty K1) T1K WFJ).
   erewrite H0 with (T1:=T1) (HK1:=HK1). eauto. 2: eapply envkv_weaken_eq_extend.
   unfold eq_rec_r, eq_rec, eq_rect.
   remember (eq_sym (splice_zero T1 (length J))). clear Heqe. dependent destruction e.
-  eauto.
-Qed.
+  eauto. *)
+Admitted.
 
-Lemma valt_subst1': forall T2 J K K1 T1K WFJ T1 (h1f : has_kind (K1 :: J) T2 K) HK1 ,
+(*
+Lemma valt_subst1': forall T2 J K K1 T1K WFJ T1 (h1f : has_kind (ext (bind_ty K1) J) T2 K) HK1 ,
   T1K = val_type HK1 WFJ ->
-  val_type h1f (envkv_cons J K1 T1K WFJ) =
+  val_type h1f (envkv_cons2 J (bind_ty K1) T1K WFJ) =
   val_type (hask_subst1' J T2 T1 K1 K h1f HK1) WFJ .
 Proof.
   intros.
@@ -1110,59 +1512,70 @@ Proof.
   unfold eq_rect. remember (splice_zero T1 (length J)).
   clear Heqe.
   dependent destruction e.
-  replace (envkv_cons J K1 T1K WFJ) with (envkv_weaken [] J K1 T1K WFJ).
+  replace (envkv_cons J (bind_ty K1) T1K WFJ) with (envkv_weaken [] J (bind_ty K1) T1K WFJ).
   erewrite H0 with (T1:=T1) (HK1:=HK1). eauto. 2: eapply envkv_weaken_eq_extend.
   unfold eq_rec_r, eq_rec, eq_rect.
   remember (eq_sym (splice_zero T1 (length J))). clear Heqe. dependent destruction e.
   eauto.
 Qed.
-
-
+*)
 
 (* ---------- env extension lemmas  ---------- *)
 
+
 Lemma envt_empty: forall W,
-    env_type [] [] [] W.
+    env_type [] [] W.
 Proof.
   intros. split. eauto. intros. inversion H.
 Qed.
 
-Lemma envt_extend: forall E G J h2 v1 T1 (h1: has_kind J T1 TStar),
-    env_type E G J h2 ->
+Lemma envt_extend: forall E (G:tenv) h2 v1 T1 (h1: has_kind G T1 TStar) vk,
+    env_type E G h2 ->
     val_type h1 h2 v1 ->
-    env_type (v1::E) (T1::G) J h2.
+    env_type (v1::E) (ext (bind_tm T1) G) (envkv_cons2 G (bind_tm T1) vk h2).
 Proof.
   intros.
   remember H as WFE. clear HeqWFE.
-  destruct H as (?&?). split. simpl. eauto.
+  destruct H as (?&?). split. rewrite ext_length. simpl. eauto.
   intros x T IX. bdestruct (x =? length G).
-  - subst x. rewrite indexr_head in IX. inversion IX. subst T1.
-    exists v1. rewrite <- H. rewrite indexr_head. eauto.
-  - rewrite indexr_skip in IX; eauto.
-    eapply WFE in IX as IX. destruct IX as (v2 & ? & ?).
-    exists v2. rewrite indexr_skip; eauto. lia.
+  - subst x. rewrite indexr_head_ext in IX. inversion IX. subst T.
+    exists v1.
+    exists (haskind_extend _ _ _ _ h1).
+    split. rewrite <- H. rewrite indexr_head. eauto.
+    eapply valt_extend in H0. eapply H0. 
+  - rewrite indexr_skip_ext in IX; eauto.
+    eapply indexr_map' in IX. destruct IX as (T' & IX & ?).
+    destruct T'. simpl in H3. inversion H3. subst. 
+    eapply WFE in IX as IX. destruct IX as (v2' & ? & ? & ?).
+    exists v2'.
+    exists (haskind_extend _ _ _ _ x0). split. 
+    rewrite indexr_skip; eauto. lia.
+    eapply valt_extend in H5. eapply H5.     
 Qed.
 
-Lemma envt_extendk: forall E G J h2 K1 (vk: val_sort K1),
-    env_type E G J h2 ->
-    env_type E (map (splice (length J) 1) G) (K1::J) (envkv_cons J K1 vk h2).
+Lemma envt_extendk: forall E G h2 K1 (vk: val_sort K1),
+    env_type E G h2 ->
+    env_type (vbool false::E) (ext (bind_ty K1) G) (envkv_cons2 G (bind_ty K1) vk h2).
 Proof.
   intros.
   remember H as WFE. clear HeqWFE.
-  destruct H as (?&?). split.
-  rewrite map_length. eauto.
-  intros x T IX.
-  eapply indexr_map' in IX. destruct IX as (T' & IX & ?).
-  eapply WFE in IX as IX. destruct IX as (v2 & ? & ? & ?).
-  exists v2. subst T.
-  exists (haskind_extend _ _ _ _ x0).
-  split. eauto.
-  edestruct valt_extend. eauto.
+  destruct H as (?&?). split. rewrite ext_length. simpl. eauto. 
+  intros x T IX. bdestruct (x =? length G).
+  - subst x. rewrite indexr_head_ext in IX. inversion IX.
+  - rewrite indexr_skip_ext in IX; eauto.
+    eapply indexr_map' in IX. destruct IX as (T' & IX & ?).
+    destruct T'. simpl in H2. inversion H2. subst. 
+    eapply WFE in IX as IX. destruct IX as (v2' & ? & ? & ?).
+    exists v2'.
+    exists (haskind_extend _ _ _ _ x0). split. 
+    rewrite indexr_skip; eauto. lia.
+    eapply valt_extend in H4. eapply H4.
 Qed.
 
 
 (* ---------- equivalence ---------- *)
 
+(*
 Lemma has_kind_subst_inverse : forall T2 J J' T1 K1 K2,
     has_kind (J'++J) (subst T2 (length J) (splice (length J) (length J') T1)) K2 ->
     has_kind J T1 K1 ->
@@ -1229,37 +1642,37 @@ Lemma eq_type_preserve_kind' : forall {J T1 T2 K},
 Proof.
   intros. specialize (eq_type_preserve_kind _ _ _ K H). intros. destruct H1; auto.
 Qed.
-
+*)
 
 (* ---------- LR compatibility lemmas  ---------- *)
 
-Lemma sem_true: forall G J,
-    sem_type G J ttrue TBool.
+Lemma sem_true: forall G,
+    sem_type G ttrue TBool.
 Proof.
   intros.
   intros E WFJ WFE.
   exists (vbool true).
-  exists (k_bool J).
+  exists (k_bool G).
   split.
   - exists 0. intros. destruct n. lia. simpl. eauto.
   - simpl. eauto.
 Qed.
 
-Lemma sem_false: forall G J,
-    sem_type G J tfalse TBool.
+Lemma sem_false: forall G,
+    sem_type G tfalse TBool.
 Proof.
   intros.
   intros E WFJ WFE.
   exists (vbool false).
-  exists (k_bool J).
+  exists (k_bool G).
   split.
   - exists 0. intros. destruct n. lia. simpl. eauto.
   - simpl. eauto.
 Qed.
 
-Lemma sem_var: forall G J x T,
-    indexr x G = Some T ->
-    sem_type G J (tvar x) T.
+Lemma sem_var: forall G x T,
+    indexr x G = Some (bind_tm T) ->
+    sem_type G (tvar x) T.
 Proof.
   intros.
   intros E WFJ WFE.
@@ -1271,29 +1684,34 @@ Proof.
   - eauto.
 Qed.
 
-Lemma sem_abs: forall G J t T1 T2,
-    sem_type (T1::G) J t T2 ->
-    has_kind J T1 TStar ->
-    has_kind J T2 TStar ->
-    sem_type G J (tabs t) (TFun T1 T2).
+Lemma sem_abs: forall G t T1 T2,
+    sem_type (ext (bind_tm T1) G) t (splice (length G) 1 T2) ->
+    has_kind G T1 TStar ->
+    has_kind G T2 TStar ->
+    sem_type G (tabs t) (TFun T1 T2).
 Proof.
-  intros ? ? ? ? ? HY W1 W2. intros E WFJ WFE.
+  intros ? ? ? ? HY W1 W2. intros E WFJ WFE.
   eexists _.
   exists (k_fun _ _ _ W1 W2).
   split.
   - exists 0. intros. destruct n. lia. simpl. eauto.
   - simpl. intros vx VX.
     edestruct HY as (vy & ? & ? & ?). eapply envt_extend; eauto.
-    specialize (hk_unique _ _ _ W2 x). intros. subst.
-    exists vy. split. eauto. eauto.
+
+    specialize (hk_unique _ _ _ (haskind_extend _ _ _ _ W2) x). intros. subst.
+                                                 
+    exists vy. split. eauto. eauto. eapply valt_extend. eauto.
+
+    Unshelve.
+    apply tt. 
 Qed.
 
-Lemma sem_app: forall G J f t T1 T2,
-    sem_type G J f (TFun T1 T2) ->
-    sem_type G J t T1 ->
-    sem_type G J (tapp f t) T2.
+Lemma sem_app: forall G f t T1 T2,
+    sem_type G f (TFun T1 T2) ->
+    sem_type G t T1 ->
+    sem_type G (tapp f t) T2.
 Proof.
-  intros ? ? ? ? ? ? HF HX. intros H WFJ WFE.
+  intros ? ? ? ? ? HF HX. intros H WFJ WFE.
   destruct (HF H WFJ WFE) as (vf & h1f & STF & VF).
   destruct (HX H WFJ WFE) as (vx & h1x & STX & VX).
   dependent destruction h1f.
@@ -1312,12 +1730,12 @@ Proof.
   - eauto.
 Qed.
 
-Lemma sem_tabs: forall G J t K1 T2,
-    sem_type (map (splice (length J) 1) G) (K1::J) t T2 ->
-    has_kind (K1::J) T2 TStar ->
-    sem_type G J (ttabs K1 t) (TAll K1 T2).
+Lemma sem_tabs: forall G t K1 T2,
+    sem_type (ext (bind_ty K1) G) t T2 ->
+    has_kind (ext (bind_ty K1) G) T2 TStar ->
+    sem_type G (ttabs K1 t) (TAll K1 T2).
 Proof.
-  intros ? ? ? ? ? HY W2. intros E WFJ WFE.
+  intros ? ? ? ? HY W2. intros E WFJ WFE.
   eexists _.
   eexists (k_all _ _ _ W2).
   split.
@@ -1329,18 +1747,18 @@ Proof.
 Qed.
 
 
-Lemma sem_tapp: forall G J t K1 T1 T2,
-    sem_type G J t (TAll K1 T2) ->
-    has_kind J T1 K1 ->
-    sem_type G J (ttapp t T1) (subst T2 (length J) T1).
+Lemma sem_tapp: forall G t K1 T1 T2,
+    sem_type G t (TAll K1 T2) ->
+    has_kind G T1 K1 ->
+    sem_type G (ttapp t T1) (subst T2 (length G) T1).
 Proof.
-  intros ? ? ? ? ? ? HF HX. intros E WFJ WFE.
+  intros ? ? ? ? ? HF HX. intros E WFJ WFE.
   destruct (HF E WFJ WFE) as (vf & h1f & STF & VF).
   dependent destruction h1f.
   destruct vf; simpl in VF; intuition.
   remember (val_type HX WFJ) as T1K.
   edestruct (VF T1K) as (vy & STY & VY).
-  exists vy.
+  exists vy. (* TODO: subst *)
   exists (hask_subst1 _ _ _ _ h1f HX).
   split.
   - destruct STF as (n1 & STF).
@@ -1361,7 +1779,7 @@ Qed.
 Lemma val_type_equiv : forall J T1 T2 K (h1: has_kind J T1 K) (h2: has_kind J T2 K) (WFJ : env_kv J),
   eq_type J T1 T2 ->
   val_type h1 WFJ = val_type h2 WFJ.
-Proof.
+Proof. (*
   intros. generalize dependent K. induction H; intros.
   - apply val_type_irrel; auto.
   - specialize (IHeq_type WFJ _ h2 h1). destruct IHeq_type. split; auto.
@@ -1386,14 +1804,16 @@ Proof.
     clear Heqe.
     dependent destruction e.
     subst t. eapply val_type_irrel.
-Qed.
+Qed.*)
+Admitted.
 
-Lemma sem_equiv: forall G J t T1 T2, eq_type J T1 T2 ->
-    has_kind J T2 TStar ->
-    sem_type G J t T1 ->
-    sem_type G J t T2.
+Lemma sem_equiv: forall G t T1 T2,
+    eq_type G T1 T2 ->
+    has_kind G T2 TStar ->
+    sem_type G t T1 ->
+    sem_type G t T2.
 Proof.
-  intros ????? KX HK HX. intros H WFJ WFE.
+  intros ???? KX HK HX. intros H WFJ WFE.
   edestruct HX as (vx & h1 & A & VX). eauto.
   eexists vx.
   exists HK.
@@ -1405,11 +1825,11 @@ Qed.
 
 (* ---------- LR fundamental property  ---------- *)
 
-Theorem fundamental: forall G J t T,
-    has_type G J t T ->
-    sem_type G J t T.
+Theorem fundamental: forall G t T,
+    has_type G t T ->
+    sem_type G t T.
 Proof.
-  intros ? ? ? ? W.
+  intros ? ? ? W.
   induction W.
   - eapply sem_true; eauto.
   - eapply sem_false; eauto.
@@ -1422,12 +1842,13 @@ Proof.
 Qed.
 
 Corollary safety: forall t T,
-  has_type [] [] t T ->
+  has_type [] t T ->
   exp_type [] [] (envkv_nil) t T.
 Proof.
   intros. eapply fundamental in H as ST; eauto.
   edestruct (ST []) as (v & ? & ? & ?). eapply envt_empty.
   exists v, x. intuition. eapply H1.
 Qed.
+
 
 End STLC.
